programs/lean/Project.lean
@@ -7,6 +7,7 @@ import Project.RustU64.Spec
 import Project.RustU64Tests.Spec
 import Project.SwapElements.Spec
 import Project.SwapElementsOpt3.Spec
+import Project.SwapElementsOpt3.Equivalence
 import Project.TotalVariation.Spec
 import Project.FloatTrunc.Spec
 import Project.FloatRound.Spec
